ifthenelse payload accessor

src/lowparse/LowParse.Low.IfThenElse.fst
@@ -122,3 +122,80 @@ let jump_ifthenelse
   if b (* eta-expansion here *)
   then vp true input pos_after_t
   else vp false input pos_after_t
+
+let clens_ifthenelse_payload
+  (#p: parse_ifthenelse_param)
+  (s: serialize_ifthenelse_param p)
+  (b: bool)
+: Tot (clens p.parse_ifthenelse_t (p.parse_ifthenelse_payload_t b))
+= {
+    clens_cond = (fun (x: p.parse_ifthenelse_t) -> p.parse_ifthenelse_tag_cond (dfst (s.serialize_ifthenelse_synth_recip x)) == b);
+    clens_get = (fun (x: p.parse_ifthenelse_t) -> dsnd (s.serialize_ifthenelse_synth_recip x) <: Ghost (p.parse_ifthenelse_payload_t b) (requires (p.parse_ifthenelse_tag_cond (dfst (s.serialize_ifthenelse_synth_recip x)) == b)) (ensures (fun _ -> True)));
+  }
+
+let gaccessor_ifthenelse_payload
+  (#p: parse_ifthenelse_param)
+  (s: serialize_ifthenelse_param p)
+  (b: bool)
+: Tot (gaccessor (parse_ifthenelse p) (dsnd (p.parse_ifthenelse_payload_parser b)) (clens_ifthenelse_payload s b))
+= fun (input: bytes) ->
+    parse_ifthenelse_eq p input;
+    let res =
+      match parse p.parse_ifthenelse_tag_parser input with
+      | Some (t, consumed) ->
+        let b = p.parse_ifthenelse_tag_cond t in
+        let input' = Seq.slice input consumed (Seq.length input) in
+        begin match parse (dsnd (p.parse_ifthenelse_payload_parser b)) input' with
+        | Some (x, _) ->
+          s.serialize_ifthenelse_synth_inverse (p.parse_ifthenelse_synth t x);
+          let (| t', x' |) = s.serialize_ifthenelse_synth_recip (p.parse_ifthenelse_synth t x) in
+          p.parse_ifthenelse_synth_injective t x t' x';
+          (consumed, Seq.length input - consumed)
+        | _ -> (consumed, Seq.length input - consumed) (* must be the same value as in the Some case, for the stateful accessor, but no postcondition here in the ghost accessor *)
+        end
+      | _ -> (0, 0) (* dummy *)
+    in
+    (res <: (res: _ { gaccessor_post' (parse_ifthenelse p) (dsnd (p.parse_ifthenelse_payload_parser b)) (clens_ifthenelse_payload s b) input res } ))
+
+inline_for_extraction
+let accessor_ifthenelse_payload'
+  (#p: parse_ifthenelse_param)
+  (s: serialize_ifthenelse_param p { p.parse_ifthenelse_tag_kind.parser_kind_subkind == Some ParserStrong  } )
+  (j: jumper p.parse_ifthenelse_tag_parser)
+  (b: bool)
+  (input: slice)
+  (pos: U32.t)
+: HST.Stack U32.t
+  (requires (fun h ->
+    (get_parser_kind (parse_ifthenelse p)).parser_kind_subkind == Some ParserStrong /\
+    (get_parser_kind (dsnd (p.parse_ifthenelse_payload_parser b))).parser_kind_subkind == Some ParserStrong /\
+    valid (parse_ifthenelse p) h input pos /\
+    (clens_ifthenelse_payload s b).clens_cond (contents (parse_ifthenelse p) h input pos)
+  ))
+  (ensures (fun h pos' h' ->
+    B.modifies B.loc_none h h' /\
+    pos' == slice_access h (gaccessor_ifthenelse_payload s b) input pos
+  ))
+= let h = HST.get () in
+  [@inline_let]
+  let _ =
+    let pos' = get_valid_pos (parse_ifthenelse p) h input pos in
+    let small = B.as_seq h (B.gsub input.base pos (pos' `U32.sub` pos)) in
+    let large = B.as_seq h (B.gsub input.base pos (input.len `U32.sub` pos)) in
+    slice_access_eq h (gaccessor_ifthenelse_payload s b) input pos;
+    valid_facts (parse_ifthenelse p) h input pos;
+    parse_ifthenelse_eq p large;
+    parse_ifthenelse_eq p small;
+    parse_strong_prefix p.parse_ifthenelse_tag_parser large small;
+    valid_facts p.parse_ifthenelse_tag_parser h input pos
+  in
+  j input pos
+
+inline_for_extraction
+let accessor_ifthenelse_payload
+  (#p: parse_ifthenelse_param)
+  (s: serialize_ifthenelse_param p { p.parse_ifthenelse_tag_kind.parser_kind_subkind == Some ParserStrong  } )
+  (j: jumper p.parse_ifthenelse_tag_parser)
+  (b: bool)
+: Tot (accessor (gaccessor_ifthenelse_payload s b))
+= accessor_ifthenelse_payload' s j b
